+++
title = "MATH 207 | Notes"
hascode = true
rss = "notes for MATH-207"
rss_title = "MATH 207 | Notes"
rss_pubdate = Date(2024, 3, 19)

tags = ["differential equations", "linear algebra"]
+++

# Differential Equations and Linear Algebra

\tableofcontents

## Linear Transformations

$T: V \rightarrow W$

$T$ is a map where $V$ is the domain and $W$ is the codomain.
Linear transformations are special types of maps.

**Definition**: A linear transformation is a function $T: V \rightarrow W$ with the properties that $T$:

- preserves scalar multiplication, $T(c\vec{v}) = cT(\vec{v})$
- preserves vector addition, $T(\vec{u}+\vec{v}) = T(\vec{u}) + T(\vec{v})$.

**Example**: $D: C^{n}(I) \rightarrow C^{n-1}(I)$, $D(f(x))=f'(x)$

Note: $I$ is an interval and $C^{n}(I)$ is a set of functions on $I$ with at least $n$ derivatives and $f^{n}(x)$ is continuous.

To prove $D$ is a linear transformation, we need to show $D$ satisfies three things:

- it is well defined
- preserves scalar multiplication
- preserves vector addition.

Step 1) Well-defined

Take $f(x)\in C^{n}(I)$. Then, $f'(x), f''(x), f'''(x), ..., f^{n}(x)$ all exist and are continuous on $I$. Therefore, $f'(x)$ exists and $f'(x)\in C^{n-1}(I)$ is equal to $f'(x)\in C^{n-1}(I)$ and is well defined.

Step 2) Scalar multiplication

Take $f(x)\in C^{n}(I)$ and $c\in\R$. Then,
\begin{align*}
D(cf(x)) &= (cf(x))'\\
         &= cf'(x)\\
         &= cD(f(x))
\end{align*}
so, $D(cf(x)) = cD(f(x))$.

Step 3) Vector addition

Take $f(x), g(x)\in C^{n}(I)$. Then,
\begin{align*}
D(f(x)+g(x)) &= (f(x)+g(x))'\\
             &= f'(x) + g'(x)\\
             &= D(f(x)) + D(g(x))
\end{align*}
so, $D(f(x)+g(x)) = D(f(x)) + D(g(x))$.

Therefore, $D$ is a linear transformation.

**Example**: $T: C^{2}(I) \rightarrow C^{0}(I), T(f(x)) = a_{2}(x)f''(x)+a_{1}f'(x)+a_{0}(x)f(x)$ where $a_{2}(x), a_{1}(x), a_{0}(x)\in C^{0}(I)$

Step 1) Well defined

$f(x), f'(x), f''(x)$ are continuous so $a_{2}(x)f''(x) + a_{1}f'(x) + a_{0}(x)f(x)$ is continuous, thus $T$ is well defined.

Step 2) Scalar multiplication

Take $f(x)\in C^{2}(I), c\in\R$.

\begin{align*}
T(cf(x)) &= a_2(x)f''(cx) + a_1f'(cx) + a_0(x)f(cx)\\
         &= ca_2(x)f''(x) + ca_1f'(x) + ca_0(x)f(x)\\
         &= c(a_2(x)f''(x) + a_1f'(x) + a_0(x)f(x))\\
         &= cT(f(x))
\end{align*}

Step 3) Vector addition

Take $f(x), g(x)\in C^{2}(I)$.

\begin{align*}
T(f(x)+g(x)) &= a_2(x)(f(x)+g(x))'' + a_1(f(x)+g(x))' + a_0(x)(f(x)+g(x))\\
             &= a_2(x)(f''(x)+g''(x)) + a_1(f'(x)+g'(x)) + a_0(x)(f(x)+g(x))\\
             &= a_2(x)f''(x) + a_2(x)g''(x) + a_1(x)f'(x) + a_1(x)g'(x) + a_0(x)f(x) + a_0(x)g(x)\\
             &= a_2(x)f''(x) + a_1(x)f'(x) + a_0(x)f(x) + a_2(x)g''(x) + a_1(x)g'(x) + a_0(x)g(x)\\
             &= T(f(x)) + T(g(x))
\end{align*}

Therefore, $T$ is a linear transformation.

**Example**: $T: \R^{2} \rightarrow \R^{2}, T((x,y)) = (x+1, y+1)$

Consider,
\begin{align*}
T((2,3)) &= (2+1,3+1)\\
         &= (3,4).
\end{align*}
Observe,
\begin{align*}
T(2(2,3)) &= T((4,6))\\
          &= (4+1,6+1)\\
          &= (5,7)
\end{align*}
and,
\begin{align*}
2T((2,3)) &= 2(3,4)\\
          &= (6,8).
\end{align*}

Since we have $T((2,3)) \neq 2T((2,3))$, $T$ doesn't preserve scalar multiplication, thus it's not a linear transformation.

**Example**: $T: \R^{2} \rightarrow \R^{2}, T((x,y)) = (x+y,x-y)$

Step 1) Scalar multiplcation

Take $(x,y)\in\R^{2}, c\in\R$.

\begin{align*}
T(c(x,y)) &= T((cx,cy))\\
          &= (cx+cy,cx-cy)\\
          &= c(x+y,x-y)\\
          &= cT(x,y)
\end{align*}

Step 2) Vector addition

Take $(x,y), (a,b)\in\R^{2}$.

\begin{align*}
T((x,y)+(a,b)) &= T((x+a,y+b))\\
               &= ((x+a)+(y+b),(x+a)-(y+b))\\
               &= (x+a+y+b,x+a-y-b)\\
               &= (x+y,x-y)+(a+b,a-b)\\
               &= T((x,y)) + T((a,b))
\end{align*}

Therefore, $T$ is a linear transformation.

**Example**: $T: \R^{2} \rightarrow \R, T(x,y) = \sqrt[3]{x^3+y^3}$

Step 1) Scalar multiplcation

Take $(x,y)\in\R^{2}, c\in\R$.

\begin{align*}
T(c(x,y)) &= T((cx,cy)))\\
          &= \sqrt[3]{(cx)^3+(cy)^3}\\
          &= \sqrt[3]{c^3(x^3+y^3)}\\
          &= c^3\sqrt[3]{x^3+y^3}\\
          &= cT((x,y))
\end{align*}

Step 2) Vector addition

Consider, $(1,0), (0,1) \in\R^{2}$.
So,
\begin{align*}
T((1,0)) &= \sqrt[3]{1^3+0^3}\\
         &= 1
\end{align*}
and,
\begin{align*}
T((0,1)) &= \sqrt[3]{0^3+1^3}\\
         &= 1.
\end{align*}
Therefore,
\begin{align*}
T((1,0)) + T((0,1)) &= 1 + 1\\
                    &= 2.
\end{align*}
Also,
\begin{align*}
T((1,0) + (0,1)) &= T((1,1))\\
                 &= \sqrt[3]{1^3+1^3}\\
                 &= \sqrt[3]{2}.
\end{align*}

Since we have $T((1,0)) + T((0,1)) \neq T((1,0) + (0,1))$, $T$ doesn't preserve vector addition, thus it's not a linear transformation.

### Linear Transformations as Matrices

Associated with any linear transformation $T, T:R^{n} \rightarrow R^{m}$, is a matrix called the matrix of $T$.

**Theorem**: If $A$ is a $m \times n$ matrix, then $T_{A}: R^{n} \rightarrow R^{m}$ defined by $T_{A}(\vec{v}) = A\vec{v}$ is a linear transformation.

**Proof**:

Step 1) Scalar multiplication
\begin{align*}
T_{A}(c\vec{v}) &= A(c\vec{v})\\
                &= cA\vec{v}\\
                &= cT_{A}(\vec{v})
\end{align*}

Step 2) Vector addition
\begin{align*}
T_{A}(\vec{u}+\vec{v}) &= A(\vec{u}+\vec{v})\\
             &= A(\vec{u}) + A(\vec{v})\\
             &= T_{A}(\vec{u}) + T_{A}(\vec{v})
\end{align*}$\blacksquare$

**Example**: Consider $A = \begin{bmatrix} 1 & 1\\ 1 & -1\end{bmatrix}$. So,

\begin{align*}
T_{A}: \R^{2} \rightarrow \R^{2}, T_{A}((x,y)) = A\begin{bmatrix} x\\ y\end{bmatrix}&=\begin{bmatrix} 1 & 1\\ 1 & -1\end{bmatrix}\begin{bmatrix}x\\ y\end{bmatrix}\\
&= \begin{bmatrix}x + y\\ x - y\end{bmatrix}\\
&= (x+y,x-y).
\end{align*}

**Example**: Consider $A = \begin{bmatrix} 2 & 1\\ 3 & 7\\ 4 & 5\end{bmatrix}$. So,

\begin{align*}
T_{A}: \R^{2} \rightarrow \R^{3}, T_{A}((x,y)) = A\begin{bmatrix}x\\ y\end{bmatrix}&=\begin{bmatrix} 2 & 1\\ 3 & 7\\ 4 & 5\end{bmatrix}\begin{bmatrix}x\\ y\end{bmatrix}\\
&= \begin{bmatrix}2x + y\\ 3x + 7y\\ 4x + 5y\end{bmatrix}\\
&= (2x+y,3x+7y,4x+5y).
\end{align*}

**Definition**: Let $T: \R^{n} \rightarrow \R^{m}$ be a linear transformation. The matrix associated with $T$ is,

\begin{equation*}
A = \begin{bmatrix}(T\vec{e}_{1}) & (T\vec{e}_{2}) & (T\vec{e}_{3}) & ... & (T\vec{e}_{n})\end{bmatrix}
\end{equation*}
where $\vec{e}_{1}, \vec{e}_{2}, \vec{e}_{3}, ..., \vec{e}_{n}$ are the standard basis vectors of $\R^{n}$.

**Example**: $T((x,y,z)) = (2x-4y+3z,7x-2z)$

\begin{align*}
A &= \begin{bmatrix}T(1,0,0) & T(0,1,0) & T(0,0,1)\end{bmatrix}\\
  &= \begin{bmatrix}2 & -4 & 3\\ 7 & 0 & -2\end{bmatrix}\\
\end{align*}

$T_{A}: \R^{3} \rightarrow \R^{2}$

\begin{align*}
T_{A}((x, y, z)) &= \begin{bmatrix}2 & -4 & 3\\ 7 & 0 & -2\end{bmatrix}\begin{bmatrix}x\\ y\\ z\end{bmatrix}\\
                 &= \begin{bmatrix}2x-4y+3z\\ 7x-2z\end{bmatrix}\\
                 &= (2x-4y+3z,7x-2z)
\end{align*}

Notice this is equal to $T$, therefore $T_{A} = T$.

### The Image and Kernel of a Linear Transformation

Observe $T: V \rightarrow W$ where $V$ is the domain and $W$ is the codomain.

**Definition**: The image of $T$ (also known as the range of $T$) is

\begin{equation*}
img(T) = \{T\vec{v}:\vec{v}\in V\}.
\end{equation*}

**Definition**: The kernel of $T$ (also known as the nullspace of $T$) is

\begin{equation*}
ker(T) = \{T\vec{v}=\vec{0}:\vec{v}\in V\}.
\end{equation*}

**Theorem**: A linear transformation must take the zero vector of $V$ to the zero vector of $W$.

**Proof**:

\begin{align*}
T(\vec{0}_{V}) &= T(0\times\vec{0}_{V})\\
               &= 0T(\vec{0}_{V})\\
               &= \vec{0}_{W}
\end{align*}$\blacksquare$

**Example**: $T((x,y)) = x^{2} + y^{2} + 1$

This is not a linear transformation because $T((0,0)) = 0 + 0 + 1 = 1$ which is not the zero vector.

**Example**: $T: M_{2}(\R) \rightarrow M_{2}(\R), T(\begin{bmatrix}a & b\\ c & d\end{bmatrix}) = \begin{bmatrix}d & c\\ b & a+1\end{bmatrix}$

This is not a linear transformation because

\begin{equation*}
T(\begin{bmatrix}0 & 0\\ 0 & 0\end{bmatrix}) = \begin{bmatrix}0 & 0\\ 0 & 1\end{bmatrix}.
\end{equation*}

Clearly, this is not the zero vector.

Observe that

\begin{align*}
ker(T) = \{T\vec{v}=\vec{0}:\vec{v}\in V\}\subseteq{V}\\
img(T) = \{T\vec{v}:\vec{v}\in V\}\subseteq{W}.
\end{align*}

**Theorem**: $ker(T)$ is a subspace of $V$.

**Proof**: W.W.T.S. three things:

- $\vec{0}\in ker(T)$
- $ker(T)$ is closed under vector addition
- $ker(T)$ is closed under scalar multiplication.

Step 1) We proved $T(\vec{0}_{V}) = \vec{0}_{W}$, so $\vec{0}\in ker(T)$.

Step 2) Take $u,v\in ker(T)$. So, $T(\vec{u})=\vec{0}$ and $T(\vec{v})=\vec{0}$. Then,

\begin{align*}
T(\vec{u}+\vec{v}) &= T(\vec{u}) + T(\vec{v})\\
                   &= \vec{0} + \vec{0}\\
                   &= \vec{0}.
\end{align*}

Thus, $\vec{u} + \vec{v} \in ker(T)$.

Step 3) Take $\vec{u}\in ker(T), c\in\R$. So, $T(\vec{u})=\vec{0}$. Then,

\begin{align*}
T(c\vec{u}) &= cT(\vec{u})\\
            &= c\vec{0}\\
            &= \vec{0}.
\end{align*}

Thus, $c\vec{u}\in ker(T)$.

$\blacksquare$

**Example**: $T: P_{2}(\R) \rightarrow \R^{2}, T(a+bx+cx^{2}) = (a-b,a+c)$

Note: $P_{2}(\R) = \{p(x) \text{is a polynomial of degree at most } 2\}$

\begin{align*}
ker(T) &= \{p(x)\in P_{2}(\R)| T(p(x)) = (0,0)\}\\
       &= \{a + ax - ax^{2}| a\in\R\}\\
       &= span\{1+x-x^{2}\}
\end{align*}

**Example**: $D: C'(I) \rightarrow C^{0}(I), D(f(x)) = f'(x)$

\begin{align*}
ker(D) &= \{f(x)\in C^{1}(I) | D(f(x))=0\}\\
       &= \{f(x)\in C^{1}(I) | f'(x)=0\}\\
       &= \{f(x)\in C^{1}(I) | f(x) = a\text{ for some } a\in\R\}
\end{align*}

**Example**: $T:C^{2}(I) \rightarrow C^{0}(I), T(f(x)) = f''(x)-f(x)$

\begin{align*}
ker(T) &= \{f\in C^{2}(I)|T(f)=0\}\\
       &= \{f\in C^{2}(I)|f''(x)-f(x)=0\}\\
       &= \{f\in C^{2}(I)|f''(x)=f(x)\}\\
       &= \{C_{1}e^{x}+C_{2}e^{-x}| C_{1}, C{2}\in\R\}
\end{align*}

## Second-Order Linear Ordinary Differential Equations

**Definition**: A second-order linear ODE is an equation of the form

\begin{equation*}
a(x)y''+b(x)y'+c(x)y=f(x)
\end{equation*}
where $a(x),b(x),c(x)$ are known as coefficient functions and $f(x)$ is known as the forcing function. This is homogeneous if $f(x)=0$, and has constant coefficients if $a(x),b(x),c(x)$ are all constant.

**Definition**: The characteristic polynomial of the second-order differential equation
\begin{equation*}
ay'' + by' + cy = 0
\end{equation*}
is the polynomial
\begin{equation*}
p(r) = ar^{2} + br + c.
\end{equation*}

### Applications

**Mass-spring system**

The equilibrium length of a mass-spring system is denoted as $l$. The distance of the mass to the system's equilibrium is denoted as $y$. The force of gravity is denoted as $F_{g}$ while the force of the spring is denoted as $F_{s}$. Respectively, $F_{g} = mg$ and $F_{s} = -k(y-l)$. So, the total force exerted on a mass in a mass-spring system is represented by the equation,

\begin{equation*}
F_{t} = -k(y-l).
\end{equation*}

However, notice that all forces are of the form $F=ma$, so

\begin{equation*}
-k(y-l) = my''.
\end{equation*}

Moving the left-hand side to the right means we have the differential equation

\begin{equation*}
my'' + k(y-l) = 0.
\end{equation*}

Let $\tilde{y} = y-l$ (relative length). Now the differential equation is

\begin{equation*}
my'' + k\tilde{y} = 0.
\end{equation*}

**Pendulum**

From the second-order differential equation

\begin{equation*}
\frac{\mathrm{d}^{2}\theta}{\mathrm{d}t^{2}} + \frac{g}{l}\sin(\theta) = 0,
\end{equation*}

we can use the small-angle approximation where $\sin(\theta) \approx \theta$ to linearize our original differential equation as

\begin{equation*}
\frac{\mathrm{d}^{2}\theta}{\mathrm{d}t^{2}} + \frac{g}{l}\theta = 0.
\end{equation*}

**LCR-circuit**

\begin{align*}
LQ'' + RQ' + \frac{1}{C}Q &= 0\\
m\tilde{y}'' + \gamma\tilde{y}' + k\tilde{y}' &= 0
\end{align*}