+++
title = "MATH 280 | Notes"
hascode = true
rss = "notes for MATH-280"
rss_title = "MATH 280 | Notes"
rss_pubdate = Date(2024, 3, 30)

tags = ["proof writing"]
+++

# Strategies of Proofs

\tableofcontents

The following will solely be proofs to exercises from Hammack's "Book of Proof".

## Direct Proof

**Exercises for Chapter 4**

Use the method of direct proof to prove the following statements.

1) If $x$ is an even integer, then $x^{2}$ is even.

**Proof**:

Let $x$ be an arbitrary integer. Suppose $x$ is even. We want to show $x^{2}$ is even. Since $x$ is even, there exists integer $j$ such that
\begin{equation*}
x = 2j.
\end{equation*}
So,
\begin{align*}
x^{2} &= (2j)^{2}\\
      &= 4j^{2}\\
      &= 2(2j^{2}).
\end{align*}
Thus, $x^{2}$ is even by definition since $2j^{2}$ is an integer.

$\blacksquare$

2. If $x$ is an odd integer, then $x^{3}$ is odd.

**Proof**:

Let $x$ be an arbitrary integer. Suppose $x$ is odd. We want to show $x^{3}$ is odd. Since $x$ is odd, there exists integer $j$ such that
\begin{equation*}
x = 2j + 1.
\end{equation*}
So,
\begin{align*}
x^{3} &= (2j+1)^{3}\\
      &= 8j^{3} + 12j^{2} + 6j + 1\\
      &= 2(4j^{3}+6j^{2}+3j) + 1.
\end{align*}
Thus, $x^{3}$ is odd by definition since $4j^{3}+6j^{2}+3j$ is an integer.

$\blacksquare$

3) If $a$ is an odd integer, then $a^{2} + 3a + 5$ is odd.

**Proof**:

Let $a$ be an arbitrary integer. Suppose $a$ is odd. We want to show $a^{2} + 3a + 5$ is odd. Since $a$ is odd, there exists integer $j$ such that
\begin{equation*}
a = 2j + 1.
\end{equation*}
So,
\begin{align*}
a^{2} + 3a + 5 &= (2j+1)^{2} + 3(2j+1) + 5\\
               &= (4j^{2}+4j+1) + (6j+3) + 5\\
               &= 4j^{2} + 10j + 9\\
               &= 2(2j^{2}+5j+4) + 1.
\end{align*}
Thus, $a^{2} + 3a + 5$ is odd by definition since $2j^{2}+5j+4$ is an integer.

$\blacksquare$

4. Suppose $x,y\in\Z$. If $x$ and $y$ are odd, then $xy$ is odd.

**Proof**:

Let $x$ and $y$ be arbitrary integers. Suppose $x$ is odd and $y$ is odd. We want to show $xy$ is odd. Since $x$ is odd, there exists integer $j$ such that
\begin{equation*}
x = 2j + 1.
\end{equation*}
Since $y$ is odd, there exists integer $k$ such that
\begin{equation*}
y = 2k + 1.
\end{equation*}
So,
\begin{align*}
xy &= (2j+1)(2k+1)\\
   &= 4jk + 2j + 2k + 1\\
   &= 2(jk+j+k) + 1.
\end{align*}
Thus, $xy$ is odd by definition since $jk+j+k$ is an integer.

$\blacksquare$

5) Suppose $x,y\in\Z$. If $x$ is even, then $xy$ is even.

**Proof**:

Let $x$ and $y$ be arbitrary integers. Suppose $x$ is even. We want to show $xy$ is even. Since $x$ is even, there exists integer $j$ such that
\begin{equation*}
x = 2j.
\end{equation*}
So,
\begin{align*}
xy &= (2j)y\\
   &= 2jy\\
   &= 2(jy).
\end{align*}
Thus, $xy$ is even by definition since $jy$ is an integer.

$\blacksquare$

6. Suppose $a,b,c\in\Z$. If $a \mid b$ and $a \mid c$, then $a \mid (b+c)$.

**Proof**:

Let $a,b$ and $c$ be arbitrary integers. Suppose $a$ divides $b$ and $a$ divides $c$. We want to show $a$ divides $b+c$. Since $a$ divides $b$, there exists integer $j$ such that
\begin{equation*}
b = aj.
\end{equation*}
Since $a$ divides $c$, there exists integer $k$ such that
\begin{equation*}
c = ak.
\end{equation*}
So,
\begin{align*}
b + c &= (aj) + (ak)\\
      &= aj + ak\\
      &= a(j+k).
\end{align*}
Thus, $a$ divides $b+c$ by definition since $j+k$ is an integer.

$\blacksquare$

7) Suppose $a,b\in\Z$. If $a \mid b$, then $a^{2} \mid b^{2}$.

**Proof**:

Let $a$ and $b$ be arbitrary integers. Suppose $a$ divides $b$. We want to show $a^{2}$ divides $b^{2}$. Since $a$ divides $b$, there exists integer $j$ such that
\begin{equation*}
b = aj.
\end{equation*}
So,
\begin{align*}
b^{2} &= (aj)^{2}\\
      &= a^{2}j^{2}\\
      &= a^{2}(j^{2}).
\end{align*}
Thus, $a^{2}$ divides $b^{2}$ by definition since $j^{2}$ is an integer.

$\blacksquare$

8. Suppose $a$ is an integer. If $5 \mid 2a$, then $5 \mid a$.

**Proof**:

Let $a$ be an arbitrary integer. Suppose $5$ divides $2a$. We want to show $5$ divides $a$. Since $5$ divides $2a$, there exists integer $j$ such that
\begin{equation*}
2a = 5j.
\end{equation*}
Notice by definition $5j$ is even.
Therefore, there exists integer $k$ such that
\begin{align*}
2a &= 5(2k)\\
   &= 10k\\
   &= 2(5k).
\end{align*}
So,
\begin{equation*}
a = 5k.
\end{equation*}
Thus, $5$ divides $a$ by definition since $k$ is an integer.

$\blacksquare$

9) Suppose $a$ is an integer. If $7 \mid 4a$, then $7 \mid a$.

**Proof**:

Let $a$ be an arbitrary integer. Suppose $7$ divides $4a$. We want to show $7$ divides $a$. Since $7$ divides $4a$, there exists integer $j$ such that
\begin{equation*}
4a = 7j.
\end{equation*}
Observe,
\begin{equation*}
2(2a) = 7j.
\end{equation*}
This means by definition $7j$ is even.
Therefore, there exists integer $k$ such that
\begin{align*}
2(2a) &= 7(2k)\\
      &= 14k\\
      &= 2(7k).
\end{align*}
So,
\begin{equation*}
2a = 7k.
\end{equation*}
Again, by definition $7k$ is even.
Therefore, there exists integer $l$ such that
\begin{align*}
2a &= 7(2l)\\
   &= 14l\\
   &= 2(7l).
\end{align*}
So,
\begin{equation*}
a = 7l.
\end{equation*}
Thus, $7$ divides $a$ by definition since $l$ is an integer.

$\blacksquare$

10. Suppose $a$ and $b$ are integers. If $a \mid b$, then $a \mid (3b^{3}-b^{2}+5b)$.

**Proof**:

Let $a$ and $b$ be arbitrary integers. Suppose $a$ divides $b$. We want to show $a$ divides $3b^{3}-b^{2}+5b$. Since $a$ divides $b$, there exists integer $j$ such that
\begin{equation*}
b = aj.
\end{equation*}
So,
\begin{align*}
3b^{3} - b^{2} + 5b &= 3(aj)^{3} - (aj)^{2} + 5(aj)\\
                    &= 3a^{3}j^{3} - a^{2}j^{2} + 5aj\\
                    &= a(3a^{2}j^{3}-aj^{2}+5j).
\end{align*}
Thus, $a$ divides $3b^{3}-b^{2}+5b$ by definition since $3a^{2}j^{3}-aj^{2}+5j$ is an integer.

$\blacksquare$

11) Suppose $a,b,c,d\in\Z$. If $a \mid b$ and $c \mid d$, then $ac \mid bd$.

**Proof**:

Let $a,b,c$ and $d$ be arbitrary integers. Suppose $a$ divides $b$ and $c$ divides $d$. We want to show $ac$ divides $bd$. Since $a$ divides $b$, there exists integer $j$ such that
\begin{equation*}
b = aj.
\end{equation*}
Since $c$ divides $d$, there exists integer $k$ such that
\begin{equation*}
d = ck.
\end{equation*}
So,
\begin{align*}
bd &= (aj)(ck)\\
   &= acjk\\
   &= ac(jk).
\end{align*}
Thus, $ac$ divides $bd$ by definition since $jk$ is an integer.

$\blacksquare$

14. If $n\in\Z$, then $5n^{2} + 3n + 7$ is odd.

**Proof**:

Let $n$ be an arbitrary integer. We want to show $5n^{2} + 3n + 7$ is odd.

**Case 1**: Suppose $n$ is even. Since $n$ is even, there exists integer $j$ such that
\begin{equation*}
n = 2j.
\end{equation*}
So,
\begin{align*}
5n^{2} + 3n + 7 &= 5(2j)^{2} + 3(2j) + 7\\
                &= 20j^{2} + 6j + 7\\
                &= 2(10j^{2}+3j+3) + 1.
\end{align*}
Observe that $10j^{2}+3j+3$ is an integer.

**Case 2**: Suppose $n$ is odd. Since $n$ is odd, there exists integer $j$ such that
\begin{equation*}
n = 2j + 1.
\end{equation*}
So,
\begin{align*}
5n^{2} + 3n + 7 &= 5(2j+1)^{2} + 3(2j+1) + 7\\
                &= (20j^{2}+20j+5) + (6j+3) + 7\\
                &= 20j^{2} + 26j + 15\\
                &= 2(10j^{2}+13j+7) + 1.
\end{align*}
Observe that $10j^{2}+13j+7$ is an integer.

In either case, $5n^{2} + 3n + 7$ is odd by definition.

$\blacksquare$

15) If $n\in\Z$, then $n^{2} + 3n + 4$ is even.

**Proof**:

Let $n$ be an arbitrary integer. We want to show $n^{2} + 3n + 4$ is even.

**Case 1**: Suppose $n$ is even. Since $n$ is even, there exists integer $j$ such that
\begin{equation*}
n = 2j.
\end{equation*}
So,
\begin{align*}
n^{2} + 3n + 4 &= (2j)^{2} + 3(2j) + 4\\
               &= 4j^{2} + 6j + 4\\
               &= 2(2j^{2}+3j+2).
\end{align*}
Observe that $2j^{2}+3j+2$ is an integer.

**Case 2**: Suppose $n$ is odd. Since $n$ is odd, there exists integer $j$ such that
\begin{equation*}
n = 2j + 1.
\end{equation*}
So,
\begin{align*}
n^{2} + 3n + 4 &= (2j+1)^{2} + 3(2j+1) + 4\\
               &= (4j^{2}+4j+1) + (6j+3) + 4\\
               &= 4j^{2} + 10j + 8\\
               &= 2(2j^{2}+5j+4).
\end{align*}
Observe that $2j^{2}+5j+4$ is an integer.

In either case, $n^{2} + 3n + 4$ is even by definition.

$\blacksquare$

16. If two integers have the same parity, then their sum is even.

**Proof**:

Let $a$ and $b$ be arbitrary integers. Suppose $a$ and $b$ have the same parity. We want to show $a + b$ is even.

**Case 1**: Suppose $a$ and $b$ are both even. Since $a$ is even, there exists integer $j$ such that
\begin{equation*}
a = 2j.
\end{equation*}
Since $b$ is even, there exists integer $k$ such that
\begin{equation*}
b = 2k.
\end{equation*}
So,
\begin{align*}
a + b &= (2j) + (2k)\\
      &= 2j + 2k\\
      &= 2(j+k).
\end{align*}
Observe that $j+k$ is an integer.

**Case 2**: Suppose $a$ and $b$ are both odd. Since $a$ is odd, there exists integer $j$ such that
\begin{equation*}
a = 2j + 1.
\end{equation*}
Since $b$ is odd, there exists integer $k$ such that
\begin{equation*}
b = 2k + 1.
\end{equation*}
So,
\begin{align*}
a + b &= (2j+1) + (2k+1)\\
      &= 2j + 1 + 2k + 1\\
      &= 2j + 2k + 2\\
      &= 2(j+k+1).
\end{align*}
Observe that $j+k+1$ is an integer.

In either case, $a + b$ is even by definition.

$\blacksquare$

17) If two integers have opposite parity, then their product is even.

**Proof**:

Let $a$ and $b$ be arbitrary integers. Without loss of generality, suppose $a$ is even and $b$ is odd. Since $a$ is even, there exists integer $j$ such that
\begin{equation*}
a = 2j.
\end{equation*}
Since $b$ is odd, there exists integer $k$ such that
\begin{equation*}
b = 2k + 1.
\end{equation*}
So,
\begin{align*}
ab &= (2j)(2k+1)\\
   &= 4jk + 2j\\
   &= 2(2jk+j).
\end{align*}
Thus, $ab$ is even by definition since $2jk+j$ is an integer.

$\blacksquare$

19. Suppose $a,b$ and $c$ are integers. If $a^{2} \mid b$ and $b^{3} \mid c$, then $a^{6} \mid c$.

**Proof**:

Let $a,b$ and $c$ be arbitrary integers. Suppose $a^{2}$ divides $b$ and $b^{3}$ divides $c$. We want to show $a^{6}$ divides $c$. Since $a^{2}$ divides $b$, there exists integer $j$ such that
\begin{equation*}
b = a^{2}j.
\end{equation*}
Since $b^{3}$ divides $c$, there exists integer $k$ such that
\begin{equation*}
c = b^{3}k.
\end{equation*}
So,
\begin{align*}
c &= (a^{2}j)^{3}k\\
  &= a^{6}j^{3}k\\
  &= a^{6}(j^{3}k).
\end{align*}
Thus, $a^{6}$ divides $c$ by definition since $j^{3}k$ is an integer.

$\blacksquare$

## Contrapositive Proof

**Exercises for Chapter 5**

Prove the following statements with contrapositive proof.

1) Suppose $n\in\Z$. If $n^{2}$ is even, then $n$ is even.

**Proof**:

We will prove the contrapositive. Let $n$ be an arbitrary integer. Suppose $n$ is odd. We want to show $n^{2}$ is odd. Since $n$ is odd, there exists integer $j$ such that
\begin{equation*}
n = 2j + 1.
\end{equation*}
So,
\begin{align*}
n^{2} &= (2j+1)^{2}\\
      &= 4j^{2} + 4j + 1\\
      &= 2(2j^{2}+2j) + 1.
\end{align*}
Thus, $n^{2}$ is odd by definition since $2j^{2}+2j$ is an integer.

$\blacksquare$

2. Suppose $n\in\Z$. If $n^{2}$ is odd, then $n$ is odd.

**Proof**:

We will prove the contrapositive. Let $n$ be an arbitrary integer. Suppose $n$ is even. We want to show $n^{2}$ is even. Since $n$ is even, there exists integer $j$ such that
\begin{equation*}
n = 2j.
\end{equation*}
So,
\begin{align*}
n^{2} &= (2j)^{2}\\
      &= 4j^{2}\\
      &= 2(2j^{2}).
\end{align*}
Thus, $n^{2}$ is even by definition since $2j^{2}$ is an integer.

$\blacksquare$

3) Suppose $a,b\in\Z$. If $a^{2}(b^{2}−2b)$ is odd, then $a$ and $b$ are odd.

**Proof**:

We will prove the contrapositive. Let $a$ and $b$ be arbitrary integers. Suppose $a$ or $b$ is even. We want to show $a^{2}(b^{2}−2b)$ is even.

**Case 1**: Suppose $a$ is even. Since $a$ is even, there exists integer $j$ such that
\begin{equation*}
a = 2j.
\end{equation*}
So,
\begin{align*}
a^{2}(b^{2}−2b) &= (2j)^{2}(b^{2}−2b)\\
                &= 4j^{2}(b^{2}−2b)\\
                &= 4b^{2}j^{2} − 8bj^{2}\\
                &= 2(2b^{2}j^{2}-4bj^{2}).
\end{align*}
Observe that $2b^{2}j^{2}-4bj^{2}$ is an integer.

**Case 2**: Suppose $b$ is even. Since $b$ is even, there exists integer $j$ such that
\begin{equation*}
b = 2j.
\end{equation*}
So,
\begin{align*}
a^{2}(b^{2}−2b) &= a^{2}((2j)^{2}−2(2j))\\
                &= a^{2}(4j^{2}−4j)\\
                &= 4a^{2}j^{2} − 4a^{2}j\\
                &= 2(2a^{2}j^{2}-2a^{2}j).
\end{align*}
Observe that $2a^{2}j^{2}-2a^{2}j$ is an integer.

**Case 3**: Suppose both $a$ and $b$ are even. Since $a$ is even, there exists integer $j$ such that
\begin{equation*}
a = 2j.
\end{equation*}
Since $b$ is even, there exists integer $k$ such that
\begin{equation*}
b = 2k.
\end{equation*}
So,
\begin{align*}
a^{2}(b^{2}−2b) &= (2j)^{2}((2k)^{2}−2(2k))\\
                &= 4j^{2}(4k^{2}−4k)\\
                &= 16j^{2}k^{2} − 16j^{2}k\\
                &= 2(8j^{2}k^{2}-8j^{2}k).
\end{align*}
Observe that $8j^{2}k^{2}-8j^{2}k$ is an integer.

Thus, no matter the case, $a^{2}(b^{2}−2b)$ is even.

$\blacksquare$

4. Suppose $a,b,c\in\Z$. If $a$ does not divide $bc$, then $a$ does not divide $b$.

**Proof**:

We will prove the contrapositive. Let $a,b$ and $c$ be arbitrary integers. Suppose $a$ divides $b$. We want to show $a$ divides $bc$. Since $a$ divides $b$, there exists integer $j$ such that
\begin{equation*}
b = aj.
\end{equation*}
So,
\begin{align*}
bc &= (aj)c\\
   &= acj\\
   &= a(cj).
\end{align*}
Thus, $a$ divides $bc$ by definition since $cj$ is an integer.

$\blacksquare$

9) Suppose $n\in\Z$. If $3 \nmid n^{2}$, then $3 \nmid n$.

**Proof**:

We will prove the contrapositive. Let $n$ be an arbitrary integer. Suppose $3$ divides $n$. We want to show $3$ divides $n^{2}$. Since $3$ divides $n$, there exists integer $j$ such that
\begin{equation*}
n = 3j.
\end{equation*}
So,
\begin{align*}
n^{2} &= (3j)^{2}\\
      &= 9j^{2}\\
      &= 3(3j^{2}).
\end{align*}
Thus, $3$ divides $n^{2}$ by definition since $3j^{2}$ is an integer.

$\blacksquare$

12. Suppose $a\in\Z$. If $a^{2}$ is not divisible by $4$, then $a$ is odd.

**Proof**:

We will prove the contrapositive. Let $a$ be an arbitrary integer. Suppose $a$ is even. We want to show $a^{2}$ is divisible by $4$. Since $a$ is even, there exists integer $j$ such that
\begin{equation*}
a = 2j.
\end{equation*}
So,
\begin{align*}
a^{2} &= (2j)^{2}\\
      &= 4j^{2}\\
      &= 4(j^{2}).
\end{align*}
Thus, $4$ divides $a^{2}$ by definition since $j^{2}$ is an integer.

$\blacksquare$

## Proof by Contradiction

**Exercises for Chapter 6**

Use the method of proof by contradiction to prove the following statements.

1) Suppose $n\in\Z$. If $n$ is odd, then $n^{2}$ is odd.

**Proof**:

By way of contradiction, suppose there exists integer $n$ such that $n$ is odd and $n^{2}$ is even. Since $n$ is odd, there exists integer $j$ such that
\begin{equation*}
n = 2j + 1.
\end{equation*}
So,
\begin{align*}
n^{2} &= (2j+1)^{2}\\
      &= 4j^{2} + 4j + 1\\
      &= 2(2j^{2}+2j) + 1.
\end{align*}
Therefore, by definition, $n^{2}$ is odd since $2j^{2}+2j$ is an integer. However, we assumed $n^{2}$ was even so this is a contradiction. Thus, $n^{2}$ is odd if $n$ is odd.

$\blacksquare$

2. Suppose $n\in\Z$. If $n^{2}$ is odd, then $n$ is odd.

**Proof**:

By way of contradiction, suppose there exists integer $n$ such that $n^{2}$ is odd and $n$ is even. Since $n$ is even, there exists integer $j$ such that
\begin{equation*}
n = 2j.
\end{equation*}
So,
\begin{align*}
n^{2} &= (2j)^{2}\\
      &= 4j^{2}\\
      &= 2(2j^{2}).
\end{align*}
Therefore, by definition, $n^{2}$ is even since $2j^{2}$ is an integer. However, we assumed $n^{2}$ was odd so this is a contradiction. Thus, $n$ is odd if $n^{2}$ is odd.

$\blacksquare$

## Mathematical Induction
